import Relation.Binary.PropositionalEquality as Eq
open Eq using (_≡_; refl)
open Eq.≡-Reasoning using (begin_; _≡⟨⟩_; _∎)

data ℕ : Set where
  zero : ℕ
  suc : ℕ → ℕ

{-# BUILTIN NATURAL ℕ #-}

_+_ : ℕ → ℕ → ℕ
zero  + n = n
suc m + n = suc (m + n)

_*_ : ℕ → ℕ → ℕ
zero  * n = zero
suc m * n = n + (m * n)

_∸_ : ℕ → ℕ → ℕ
m     ∸ zero  = m
zero  ∸ suc n = zero
suc m ∸ suc n = m ∸ n

infixl 6  _+_  _∸_
infixl 7  _*_

{-# BUILTIN NATPLUS _+_ #-}
{-# BUILTIN NATTIMES _*_ #-}
{-# BUILTIN NATMINUS _∸_ #-}


data Bin : Set where
  ⟨⟩ : Bin
  _O : Bin → Bin
  _I : Bin → Bin

inc : Bin → Bin
inc ⟨⟩    = ⟨⟩ I
inc (s O) = s I
inc (s I) = (inc s) O


to : ℕ → Bin
to zero = ⟨⟩ O
to (suc n) = inc (to n)

from : Bin → ℕ
from ⟨⟩ = zero
from (s O) = from s * 2
from (s I) = from s * 2 + 1
